Made ticketlock an instance of FairLock interface

fairness/examples/ticketlock/ext_models.v
@@ -1,44 +1,46 @@
 From trillium.fairness Require Import fairness fair_termination.
-From trillium.fairness.examples.ticketlock Require Import set_map_properties.
+From trillium.fairness.examples.ticketlock Require Import set_map_properties trace_helpers. 
+
+Class ExtModel := {
+  innerM: FairModel;
+  EI: Type; (* indexes over external transitions *)
+  DecEI: EqDecision EI;
+  CntEI: Countable EI;
+  ETs: EI -> relation (fmstate innerM);
+  (* Ensures that in any state there is only a finite amount 
+     of possible external transitions, even if EI is infinite *)
+  active_exts: fmstate (innerM) -> gset EI;
+  active_exts_spec: forall st ι, ι ∈ active_exts st <-> ∃ st', ETs ι st st';
+}. 
 
 (* TODO: can it be generalized to Model? *)
 Section ExtModels.
-  Context (M: FairModel).
-  
-  Context {EI: Type}. (* indexes over external transitions *)
-  Context {DecEI: EqDecision EI} {CntEI: Countable EI}.
-  Context (ETs: EI -> relation (fmstate M)). 
-
-  (* Ensures that in any state there is only a finite amount 
-     of possible external transitions, even if EI is infinite *)
-  Context (active_exts: fmstate M -> gset EI). 
-  Hypothesis (active_exts_spec: forall st ι, ι ∈ active_exts st <-> ∃ st', ETs ι st st').
-
+  Context (EM: ExtModel). 
 
   Inductive env_role := env (i: EI).
-  Definition ext_role: Type := (fmrole M + env_role). 
+  Definition ext_role: Type := (fmrole innerM + env_role). 
 
   Global Instance env_role_EqDec: EqDecision env_role. 
-  Proof using -DecEI. clear -DecEI. solve_decision. Qed. 
+  Proof using. generalize DecEI. solve_decision. Qed. 
 
   Global Instance env_role_cnt: Countable env_role. 
-  Proof.
-    refine {| 
+  Proof using.
+    unshelve refine {| 
         encode r := match r with | env i => encode i end;
         decode i := match (decode i) with | Some r => Some (env r) | None => None end
-      |}.
+      |}; try by apply EM. 
     intros. destruct x.
     by rewrite decode_encode.
   Qed.
 
-  Inductive ext_trans: fmstate M -> option ext_role -> fmstate M -> Prop :=
-  | ext_model_step s1 ρ s2 (STEP: fmtrans M s1 (Some ρ) s2):
+  Inductive ext_trans: fmstate innerM -> option ext_role -> fmstate innerM -> Prop :=
+  | ext_model_step s1 ρ s2 (STEP: fmtrans innerM s1 (Some ρ) s2):
     ext_trans s1 (Some (inl ρ)) s2
   | ext_ext_step s1 s2 ι (REL: ETs ι s1 s2):
     ext_trans s1 (Some (inr (env ι))) s2. 
 
-  Definition ext_live_roles (st: fmstate M): gset ext_role :=
-    set_map inl (live_roles M st) ∪
+  Definition ext_live_roles (st: fmstate innerM): gset ext_role :=
+    set_map inl (live_roles innerM st) ∪
     set_map (inr ∘ env) (active_exts st). 
 
   Lemma ext_live_spec:
@@ -49,21 +51,24 @@ Section ExtModels.
     - apply elem_of_union_l. apply elem_of_map_2. 
       eapply fm_live_spec; eauto. 
     - apply elem_of_union_r.
-      rewrite set_map_compose_gset. 
+      unshelve erewrite set_map_compose_gset; [apply EM| ]. 
       do 2 apply elem_of_map_2.
       apply active_exts_spec. eauto.
   Qed.
   
-  Definition ext_model: FairModel.
+  Definition ext_model_FM: FairModel.
   Proof using All. 
     refine({|
-              fmstate := fmstate M;
+              fmstate := fmstate innerM;
               fmrole := ext_role;
               fmtrans := ext_trans;
               live_roles := ext_live_roles;
               fm_live_spec := ext_live_spec
             |}).
-    apply M. 
+    apply innerM. 
   Defined.
+
+  Definition inner_fair_ext_model_trace :=
+    set_fair_model_trace (λ ρ0: fmrole ext_model_FM, ∃ r, ρ0 = inl r).
 
 End ExtModels. 
