fairness/examples/ticketlock/fair_lock.v
@@ -1,0 +1,62 @@
+From iris.proofmode Require Import tactics.
+From trillium.fairness Require Import fairness fair_termination.
+From trillium.fairness.examples.ticketlock Require Import lemmas trace_len set_map_properties ext_models trace_helpers. 
+
+
+Section FairLock.
+  Context (EM: ExtModel). 
+
+  Let m := @innerM EM. 
+  Let St := fmstate m.
+  Let R := fmrole m.
+  Let EFM := ext_model_FM EM. 
+
+  Context (can_lock_st can_unlock_st has_lock_st active_st: R -> St -> Prop).
+  Context {active_st_Dec: forall ρ st, Decision (active_st ρ st)}. 
+  Context (is_init_st: St -> Prop). 
+  
+
+  Definition eventual_release (tr: mtrace EFM) (ρ: R) (i: nat) :=
+    forall (ρ': R) j st' (JTH: tr S!! j = Some st')
+      (HAS_LOCK: has_lock_st ρ' st')
+      (PREVr: ρ' = ρ -> j < i),
+    exists k st'', tr S!! k = Some st'' /\ j <= k /\ active_st ρ' st''.
+
+  Lemma eventual_release_strenghten tr ρ i
+    (EV_REL: eventual_release tr ρ i):
+    forall ρ' j st' (JTH: tr S!! j = Some st')
+      (HAS_LOCK: has_lock_st ρ' st')
+      (PREVr: ρ' = ρ -> j < i),
+    exists k, ClassicalFacts.Minimal 
+           (fun k => exists st'', tr S!! k = Some st'' /\ j <= k /\ active_st ρ' st'') k.
+  Proof using active_st_Dec. 
+    intros. red in EV_REL. specialize (EV_REL _ _ _ JTH HAS_LOCK PREVr).
+    destruct EV_REL as [k EV_REL]. pattern k in EV_REL. 
+    eapply min_prop_dec in EV_REL; eauto.
+    intros.
+    destruct (tr S!! n) as [st | ] eqn:NTH.
+    2: { right. intros (? & ? & ?). congruence. }
+    destruct (decide (j <= n)).
+    2: { right. intros (? & ? & ?). lia. }
+    destruct (active_st_Dec ρ' st).
+    - left. eauto.
+    - right. intros (? & ? & ? & ?). congruence.
+  Qed.
+
+  Definition fair_lock_progress :=
+    forall (tr: mtrace EFM) (ρ: R) (i: nat) (st: St)
+      (VALID: mtrace_valid tr)
+      (FROM_INIT: forall st0, tr S!! 0 = Some st0 -> is_init_st st0)
+      (FAIR: inner_fair_ext_model_trace EM tr)
+      (ITH: tr S!! i = Some st)
+      (CAN_LOCK: can_lock_st ρ st)
+      (ACT: active_st ρ st)
+      (EV_REL: forall j (LE: i <= j), eventual_release tr ρ j),
+    exists n st', i < n /\ tr S!! n = Some st' /\ has_lock_st ρ st' /\ ¬ active_st ρ st'.
+
+      
+  Class FairLock := {
+      lock_progress: fair_lock_progress
+  }.
+
+End FairLock.
